Stlc/Lemmas.v
@@ -1,5 +1,3 @@
-From Coq Require Import ssreflect ssrfun ssrbool.
-
 Require Import Coq.Logic.FunctionalExtensionality.
 Require Import Coq.Program.Equality.
 Require Import Program.
@@ -19,103 +17,8 @@ Require Import Lia.
 
 Require Export Stlc.Definitions.
 
-(** NOTE: Auxiliary theorems are hidden in generated documentation.
-    In general, there is a [_rec] version of every lemma involving
-    [open] and [close]. *)
-
-(* begin hide *)
-
-(* *********************************************************************** *)
-(** * Induction principles for nonterminals *)
-
-(*
-Scheme typ_ind' := Induction for typ Sort Prop.
-
-Definition typ_mutind :=
-  fun H1 H2 H3 =>
-  typ_ind' H1 H2 H3.
-
-Scheme typ_rec' := Induction for typ Sort Set.
-
-Definition typ_mutrec :=
-  fun H1 H2 H3 =>
-  typ_rec' H1 H2 H3.
-
-Scheme exp_ind' := Induction for exp Sort Prop.
-
-Definition exp_mutind :=
-  fun H1 H2 H3 H4 H5 =>
-  exp_ind' H1 H2 H3 H4 H5.
-
-Scheme exp_rec' := Induction for exp Sort Set.
-
-Definition exp_mutrec :=
-  fun H1 H2 H3 H4 H5 =>
-  exp_rec' H1 H2 H3 H4 H5.
-*)
-
-(* end hide *)
-
-(* *********************************************************************** *)
-(** * Close *)
 
 
-(* *********************************************************************** *)
-(** * Degree *)
-
-(* subsumed by the indexed representation. *)
-
-(*
-(** These define only an upper bound, not a strict upper bound. *)
-
-Inductive degree_exp_wrt_exp {n} : nat -> exp n -> Prop :=
-  | degree_wrt_exp_abs : forall n1 e1,
-    degree_exp_wrt_exp (S n1) e1 ->
-    degree_exp_wrt_exp n1 (abs e1)
-  | degree_wrt_exp_var_f : forall n1 x1,
-    degree_exp_wrt_exp n1 (var_f x1)
-  | degree_wrt_exp_var_b : forall n1 n2,
-      forall pf, lt n2 n1 ->
-    degree_exp_wrt_exp n1 (var_b pf)
-  | degree_wrt_exp_app : forall n1 e1 e2,
-    degree_exp_wrt_exp n1 e1 ->
-    degree_exp_wrt_exp n1 e2 ->
-    degree_exp_wrt_exp n1 (app e1 e2).
-
-Scheme degree_exp_wrt_exp_ind' := Induction for degree_exp_wrt_exp Sort Prop.
-
-Definition degree_exp_wrt_exp_mutind :=
-  fun H1 H2 H3 H4 H5 =>
-  degree_exp_wrt_exp_ind' H1 H2 H3 H4 H5.
-
-#[global] Hint Constructors degree_exp_wrt_exp : core lngen.
-*)
-
-(* begin hide *)
-
-(* *********************************************************************** *)
-(** * Local closure (induction principles) *)
-(*
-
-Scheme lc_exp_ind' := Induction for lc_exp Sort Prop.
-
-Definition lc_exp_mutind :=
-  fun H1 H2 H3 H4 =>
-  lc_exp_ind' H1 H2 H3 H4.
-
-#[global] Hint Constructors lc_exp : core lngen.
-*)
-(* end hide *)
-
-
-(* *********************************************************************** *)
-(** * Body *)
-
-(*
-Definition body_exp_wrt_exp e1 := forall x1, lc_exp (open_exp_wrt_exp e1 (var_f x1)).
-
-#[global] Hint Unfold body_exp_wrt_exp.
-*)
 
 (* *********************************************************************** *)
 (** * Tactic support *)
@@ -124,8 +27,20 @@ Definition body_exp_wrt_exp e1 := forall x1, lc_exp (open_exp_wrt_exp e1 (var_f 
 
 #[global] Hint Resolve @plus_le_compat : lngen.
 
-(** Redefine some tactics. *)
+Ltac destruct_option :=
+  let rec main x :=
+    let h := fresh "EQ" in
+    match type of x with
+      | option _ => destruct x eqn:h
+    end
+  in
+  match goal with
+    | |- context [?x] => main x
+    | H : _ |- _ => main H
+    | _ : context [?x] |- _ => main x
+  end.
 
+(** Redefine some tactics. *)
 
 Ltac default_case_split ::=
   first
@@ -133,6 +48,9 @@ Ltac default_case_split ::=
     | progress destruct_sum
     | progress safe_f_equal
     ].
+
+Ltac default_auto ::= auto with arith lngen; tauto.
+Ltac default_autorewrite ::= simp_stlc.
 
 
 (* *********************************************************************** *)
@@ -155,7 +73,6 @@ Lemma fv_exp_weaken_exp :
 (forall n1 (e1 : exp n1),
   fv_exp (weaken_exp e1) = fv_exp e1).
 Proof. 
-
   intros n1 e1.
   funelim (weaken_exp e1); program_simpl.
 Qed.
@@ -167,1298 +84,406 @@ Hint Rewrite fv_exp_weaken_exp : weaken_exp.
 (* *********************************************************************** *)
 (** * Theorems about [size] *)
 
-Ltac default_auto ::= auto with arith lngen; tauto.
-Ltac default_autorewrite ::= fail.
-
-
-(* begin hide *)
-
-(*
-Lemma size_typ_min_mutual :
-(forall T1, 1 <= size_typ T1).
-Proof.
-intros T1. induction T1; default_simp.
-Qed.
-
-(* end hide *)
-
-Lemma size_typ_min :
-forall T1, 1 <= size_typ T1.
-Proof.
-pose proof size_typ_min_mutual as H; intuition eauto.
-Qed.
-
-#[global] Hint Resolve size_typ_min : lngen.
-*)
-
-(* begin hide *)
-
-Lemma size_exp_min_mutual :
-(forall {n} (e1 : exp n), 1 <= size_exp e1).
-Proof.
-  move=>n e1.  dependent induction e1; default_simp.  
-Admitted. (* lia ??? *)
-
-(* end hide *)
-
 Lemma size_exp_min :
-forall {n} (e1:exp n), 1 <= size_exp e1.
+(forall n (e1 : exp n), 1 <= size_exp e1).
 Proof.
-move=>n.
-pose proof (@size_exp_min_mutual n) as H; intuition eauto.
-Qed.
+  intros n e1.  dependent induction e1; default_simp.  
+Admitted. (* lia ??? *)
 
 #[global] Hint Resolve size_exp_min : lngen.
 
-(* begin hide *)
-
-Lemma size_exp_close_exp_wrt_exp_rec_mutual :
-(forall {n1} (e1 : exp n1) x1,
-  size_exp (close_exp_wrt_exp_rec x1 e1) = size_exp e1).
+Lemma size_exp_close_exp_wrt_exp :
+(forall n1 (e1 : exp n1) x1,
+  size_exp (close_exp_wrt_exp x1 e1) = size_exp e1).
 Proof.
-move=> n1 e1 x1.  
-funelim (close_exp_wrt_exp_rec x1 e1); program_simpl; simp close_exp_wrt_exp_rec. 
-default_simp. 
+intros n1 e1 x1.  
+funelim (close_exp_wrt_exp x1 e1); default_simp. 
 Qed.
 
-
-(* end hide *)
-
-Lemma size_exp_open_exp_wrt_exp_rec_mutual :
-(forall k (e1 : exp (S k)) (e2 : exp k),
-  size_exp e1 <= size_exp (open_exp_wrt_exp_rec e2 e1)).
-Proof.
-intros k e1 e2.
-apply_funelim (open_exp_wrt_exp_rec e2 e1); default_simp; try lia; eauto with lngen.
-Admitted.
-
-Lemma size_exp_open_exp_wrt_exp_rec :
-forall k (e1 : exp (S k)) (e2 : exp k),
-  size_exp e1 <= size_exp (open_exp_wrt_exp_rec e2 e1).
-Proof.
-pose proof size_exp_open_exp_wrt_exp_rec_mutual as H; intuition eauto.
-Qed.
-
-#[global] Hint Resolve size_exp_open_exp_wrt_exp_rec : lngen.
-
-(* end hide *)
+#[global] Hint Resolve size_exp_close_exp_wrt_exp : lngen.
 
 Lemma size_exp_open_exp_wrt_exp :
-forall e1 e2,
-  size_exp e1 <= size_exp (open_exp_wrt_exp e1 e2).
+(forall k (e1 : exp (S k)) (e2 : exp k),
+  size_exp e1 <= size_exp (open_exp_wrt_exp e2 e1)).
 Proof.
-unfold open_exp_wrt_exp; default_simp. 
-Qed.
-
-#[global] Hint Resolve size_exp_open_exp_wrt_exp : lngen.
-
-
-Lemma size_exp_open_exp_wrt_exp_rec_var_mutual :
-(forall k ( e1 : exp (S k)) x1,
-  size_exp (open_exp_wrt_exp_rec (var_f x1) e1) = size_exp e1).
-Proof.
-intros k e1 x1.
-dependent induction e1; simp_stlc; default_simp.
-destruct decrease_fin; default_simp.
-Qed.
-
-Lemma size_exp_open_exp_wrt_exp_rec_var :
-forall k (e1 : exp (S k)) x1 ,
-  size_exp (open_exp_wrt_exp_rec (var_f x1) e1) = size_exp e1.
-Proof.
-pose proof size_exp_open_exp_wrt_exp_rec_var_mutual as H; intuition eauto.
-Qed.
-#[global] Hint Resolve size_exp_open_exp_wrt_exp_rec_var : lngen.
-Hint Rewrite size_exp_open_exp_wrt_exp_rec_var using solve [auto] : lngen.
-
-(* end hide *)
+intros k e1 e2.
+funelim (open_exp_wrt_exp e2 e1); default_simp; try lia; eauto with lngen.
+Admitted.
 
 Lemma size_exp_open_exp_wrt_exp_var :
-forall (e1 : exp 1) x1,
-  size_exp (open_exp_wrt_exp e1 (var_f x1)) = size_exp e1.
+(forall k (e : exp (S k)) x,
+  size_exp (open_exp_wrt_exp (var_f x) e) = size_exp e).
 Proof.
-  simp_stlc; default_simp. 
+intros k e x.
+dependent induction e; default_simp. destruct_option; default_simp.
 Qed.
 
 #[global] Hint Resolve size_exp_open_exp_wrt_exp_var : lngen.
 Hint Rewrite size_exp_open_exp_wrt_exp_var using solve [auto] : lngen.
 
 (* *********************************************************************** *)
-(** * Theorems about [degree] *)
-(*
-Ltac default_auto ::= auto with lngen; tauto.
-Ltac default_autorewrite ::= fail.
-
-(* begin hide *)
-
-Lemma degree_exp_wrt_exp_S_mutual :
-(forall n1 e1,
-  degree_exp_wrt_exp n1 e1 ->
-  degree_exp_wrt_exp (S n1) e1).
-Proof.
-apply_mutual_ind degree_exp_wrt_exp_mutind;
-default_simp.
-Qed.
-
-(* end hide *)
-
-Lemma degree_exp_wrt_exp_S :
-forall n1 e1,
-  degree_exp_wrt_exp n1 e1 ->
-  degree_exp_wrt_exp (S n1) e1.
-Proof.
-pose proof degree_exp_wrt_exp_S_mutual as H; intuition eauto.
-Qed.
-
-#[global] Hint Resolve degree_exp_wrt_exp_S : lngen.
-
-Lemma degree_exp_wrt_exp_O :
-forall n1 e1,
-  degree_exp_wrt_exp O e1 ->
-  degree_exp_wrt_exp n1 e1.
-Proof.
-induction n1; default_simp.
-Qed.
-
-#[global] Hint Resolve degree_exp_wrt_exp_O : lngen.
-
-(* begin hide *)
-
-Lemma degree_exp_wrt_exp_close_exp_wrt_exp_rec_mutual :
-(forall e1 x1 n1,
-  degree_exp_wrt_exp n1 e1 ->
-  degree_exp_wrt_exp (S n1) (close_exp_wrt_exp_rec n1 x1 e1)).
-Proof.
-apply_mutual_ind exp_mutind;
-default_simp.
-Qed.
-
-(* end hide *)
-
-(* begin hide *)
-
-Lemma degree_exp_wrt_exp_close_exp_wrt_exp_rec :
-forall e1 x1 n1,
-  degree_exp_wrt_exp n1 e1 ->
-  degree_exp_wrt_exp (S n1) (close_exp_wrt_exp_rec n1 x1 e1).
-Proof.
-pose proof degree_exp_wrt_exp_close_exp_wrt_exp_rec_mutual as H; intuition eauto.
-Qed.
-
-#[global] Hint Resolve degree_exp_wrt_exp_close_exp_wrt_exp_rec : lngen.
-
-(* end hide *)
-
-Lemma degree_exp_wrt_exp_close_exp_wrt_exp :
-forall e1 x1,
-  degree_exp_wrt_exp 0 e1 ->
-  degree_exp_wrt_exp 1 (close_exp_wrt_exp x1 e1).
-Proof.
-unfold close_exp_wrt_exp; default_simp.
-Qed.
-
-#[global] Hint Resolve degree_exp_wrt_exp_close_exp_wrt_exp : lngen.
-
-(* begin hide *)
-
-Lemma degree_exp_wrt_exp_close_exp_wrt_exp_rec_inv_mutual :
-(forall e1 x1 n1,
-  degree_exp_wrt_exp (S n1) (close_exp_wrt_exp_rec n1 x1 e1) ->
-  degree_exp_wrt_exp n1 e1).
-Proof.
-apply_mutual_ind exp_mutind;
-default_simp; eauto with lngen.
-Qed.
-
-(* end hide *)
-
-(* begin hide *)
-
-Lemma degree_exp_wrt_exp_close_exp_wrt_exp_rec_inv :
-forall e1 x1 n1,
-  degree_exp_wrt_exp (S n1) (close_exp_wrt_exp_rec n1 x1 e1) ->
-  degree_exp_wrt_exp n1 e1.
-Proof.
-pose proof degree_exp_wrt_exp_close_exp_wrt_exp_rec_inv_mutual as H; intuition eauto.
-Qed.
-
-Hint Immediate degree_exp_wrt_exp_close_exp_wrt_exp_rec_inv : lngen.
-
-(* end hide *)
-
-Lemma degree_exp_wrt_exp_close_exp_wrt_exp_inv :
-forall e1 x1,
-  degree_exp_wrt_exp 1 (close_exp_wrt_exp x1 e1) ->
-  degree_exp_wrt_exp 0 e1.
-Proof.
-unfold close_exp_wrt_exp; eauto with lngen.
-Qed.
-
-Hint Immediate degree_exp_wrt_exp_close_exp_wrt_exp_inv : lngen.
-
-(* begin hide *)
-
-Lemma degree_exp_wrt_exp_open_exp_wrt_exp_rec_mutual :
-(forall e1 e2 n1,
-  degree_exp_wrt_exp (S n1) e1 ->
-  degree_exp_wrt_exp n1 e2 ->
-  degree_exp_wrt_exp n1 (open_exp_wrt_exp_rec n1 e2 e1)).
-Proof.
-apply_mutual_ind exp_mutind;
-default_simp.
-Qed.
-
-(* end hide *)
-
-(* begin hide *)
-
-Lemma degree_exp_wrt_exp_open_exp_wrt_exp_rec :
-forall e1 e2 n1,
-  degree_exp_wrt_exp (S n1) e1 ->
-  degree_exp_wrt_exp n1 e2 ->
-  degree_exp_wrt_exp n1 (open_exp_wrt_exp_rec n1 e2 e1).
-Proof.
-pose proof degree_exp_wrt_exp_open_exp_wrt_exp_rec_mutual as H; intuition eauto.
-Qed.
-
-#[global] Hint Resolve degree_exp_wrt_exp_open_exp_wrt_exp_rec : lngen.
-
-(* end hide *)
-
-Lemma degree_exp_wrt_exp_open_exp_wrt_exp :
-forall e1 e2,
-  degree_exp_wrt_exp 1 e1 ->
-  degree_exp_wrt_exp 0 e2 ->
-  degree_exp_wrt_exp 0 (open_exp_wrt_exp e1 e2).
-Proof.
-unfold open_exp_wrt_exp; default_simp.
-Qed.
-
-#[global] Hint Resolve degree_exp_wrt_exp_open_exp_wrt_exp : lngen.
-
-(* begin hide *)
-
-Lemma degree_exp_wrt_exp_open_exp_wrt_exp_rec_inv_mutual :
-(forall e1 e2 n1,
-  degree_exp_wrt_exp n1 (open_exp_wrt_exp_rec n1 e2 e1) ->
-  degree_exp_wrt_exp (S n1) e1).
-Proof.
-apply_mutual_ind exp_mutind;
-default_simp; eauto with lngen.
-Qed.
-
-(* end hide *)
-
-(* begin hide *)
-
-Lemma degree_exp_wrt_exp_open_exp_wrt_exp_rec_inv :
-forall e1 e2 n1,
-  degree_exp_wrt_exp n1 (open_exp_wrt_exp_rec n1 e2 e1) ->
-  degree_exp_wrt_exp (S n1) e1.
-Proof.
-pose proof degree_exp_wrt_exp_open_exp_wrt_exp_rec_inv_mutual as H; intuition eauto.
-Qed.
-
-Hint Immediate degree_exp_wrt_exp_open_exp_wrt_exp_rec_inv : lngen.
-
-(* end hide *)
-
-Lemma degree_exp_wrt_exp_open_exp_wrt_exp_inv :
-forall e1 e2,
-  degree_exp_wrt_exp 0 (open_exp_wrt_exp e1 e2) ->
-  degree_exp_wrt_exp 1 e1.
-Proof.
-unfold open_exp_wrt_exp; eauto with lngen.
-Qed.
-
-Hint Immediate degree_exp_wrt_exp_open_exp_wrt_exp_inv : lngen.
-*)
-
-
-(* *********************************************************************** *)
 (** * Theorems about [open] and [close] *)
 
 Ltac default_auto ::= auto with lngen brute_force; tauto.
-Ltac default_autorewrite ::= fail.
+Ltac default_autorewrite ::= simp_stlc.
 
-(* begin hide *)
+Ltac noconf_exp := 
+  match goal with 
+    | [ H : var_b _ = var_b _ |- _ ] => noconf H
+    | [ H : var_f _ = var_f _ |- _ ] => noconf H
+    | [ H : abs _ = abs _ |- _ ] => noconf H
+    | [ H : app _ _ = app _ _ |- _ ] => noconf H
+  end.
 
-Lemma close_exp_wrt_exp_rec_inj_mutual :
+Lemma close_exp_wrt_exp_inj :
 (forall k (e1 : exp k) e2 x1,
-  close_exp_wrt_exp_rec x1 e1 = close_exp_wrt_exp_rec x1 e2 ->
+  close_exp_wrt_exp x1 e1 = close_exp_wrt_exp x1 e2 ->
   e1 = e2).
 Proof.
   intros k e1 e2 x1.
-  funelim (close_exp_wrt_exp_rec x1 e1).
-  all: program_simpl.
+  funelim (close_exp_wrt_exp x1 e1).
+  all: default_simp.
   all: match goal with
           | |- _ = ?term => destruct term
-        end;
-     simp close_exp_wrt_exp_rec in H;
-     noconf H.
+        end.
+  all: try simp close_exp_wrt_exp in H.
+  all: try noconf_exp.
   all: try discriminate.
-  all: try simp close_exp_wrt_exp_rec in *.
+  all: try simp close_exp_wrt_exp in *.
   all: try (destruct (x1 == x); simpl in H; try discriminate).
-  + apply increase_fin_inj in H. rewrite H. auto.
-  + noconf H. symmetry in H.
-    move: (increase_not_n f) => h. done.
-  + noconf H. move: (increase_not_n f) => h. done.
-  + destruct (x1 == x0); subst; simpl in H; try discriminate; auto.
-  + destruct (x1 == x0); subst; simpl in H; try discriminate; auto.
-    noconf H. auto.
-  + noconf H0. f_equal. eapply H. auto.
-  + noconf H1. f_equal. eapply H. eauto. eapply H0. eauto.
-Qed.
-
-Lemma close_exp_wrt_exp_rec_inj :
-forall k (e1 e2 : exp k) x1,
-  close_exp_wrt_exp_rec x1 e1 = close_exp_wrt_exp_rec x1 e2 ->
-  e1 = e2.
-Proof.
-pose proof close_exp_wrt_exp_rec_inj_mutual as H; intuition eauto.
-Qed.
-
-Hint Immediate close_exp_wrt_exp_rec_inj : lngen.
-
-(* end hide *)
-
-Lemma close_exp_wrt_exp_inj :
-forall (e1 e2 : exp 0) x1,
-  close_exp_wrt_exp x1 e1 = close_exp_wrt_exp x1 e2 ->
-  e1 = e2.
-Proof.
-unfold close_exp_wrt_exp; eauto with lngen.
+  all: try noconf_exp; default_simp.
+  + eapply increase_fin_inj; eauto.  
+  + exfalso. eapply increase_not_n; eauto.
+  + exfalso. eapply increase_not_n; eauto.  
 Qed.
 
 Hint Immediate close_exp_wrt_exp_inj : lngen.
 
-(* begin hide *)
-
-
-Lemma close_exp_wrt_exp_rec_open_exp_wrt_exp_rec_mutual :
-(forall {n1} (e1 : exp (S n1)) x1 ,
+Lemma close_exp_wrt_exp_open_exp_wrt_exp :
+(forall n1 (e1 : exp (S n1)) x1 ,
   x1 `notin` fv_exp e1 ->
-  close_exp_wrt_exp_rec x1 (open_exp_wrt_exp_rec (var_f x1) e1) = e1).
+  close_exp_wrt_exp x1 (open_exp_wrt_exp (var_f x1) e1) = e1).
 Proof.
 intros. 
 dependent induction e1.
-all: simp open_exp_wrt_exp_rec.
-all: simp close_exp_wrt_exp_rec.
-+ destruct (decrease_fin n1 f) eqn:E1.
-  ++ simp close_exp_wrt_exp_rec. f_equal.
-  eauto using decrease_increase_fin.
-  ++ simp weaken. simp close_exp_wrt_exp_rec.
-     rewrite eq_dec_refl. simpl.
-     f_equal. eauto using decrease_to_fin.
-+ destruct (x1 == x); subst; simpl. simpl in H. fsetdec. auto.
-+ f_equal.
-  rewrite IHe1; eauto.
-+ simpl in H. f_equal. rewrite IHe1_1; eauto. rewrite IHe1_2; eauto.
-Qed.
-
-(* end hide *)
-
-(* begin hide *)
-
-Lemma close_exp_wrt_exp_rec_open_exp_wrt_exp_rec :
-forall {n1} (e1:exp (S n1)) x1,
-  x1 `notin` fv_exp e1 ->
-  close_exp_wrt_exp_rec x1 (open_exp_wrt_exp_rec (var_f x1) e1) = e1.
-Proof.
-intro n1.
-pose proof (@close_exp_wrt_exp_rec_open_exp_wrt_exp_rec_mutual n1) as H; intuition eauto.
-Qed.
-
-#[global] Hint Resolve close_exp_wrt_exp_rec_open_exp_wrt_exp_rec : lngen.
-(* Hint Rewrite close_exp_wrt_exp_rec_open_exp_wrt_exp_rec using solve [auto] : lngen. *)
-
-(* end hide *)
-
-Lemma close_exp_wrt_exp_open_exp_wrt_exp :
-forall (e1 : exp 1) x1,
-  x1 `notin` fv_exp e1 ->
-  close_exp_wrt_exp x1 (open_exp_wrt_exp e1 (var_f x1)) = e1.
-Proof.
-unfold close_exp_wrt_exp; unfold open_exp_wrt_exp; default_simp.
+all: simp_stlc.
+all: default_simp.
+destruct decrease_fin eqn:EQ; default_simp. 
+eauto using decrease_increase_fin.
+eauto using decrease_to_fin.
 Qed.
 
 #[global] Hint Resolve close_exp_wrt_exp_open_exp_wrt_exp : lngen.
-Hint Rewrite close_exp_wrt_exp_open_exp_wrt_exp using solve [auto] : lngen.
+Hint Rewrite close_exp_wrt_exp_open_exp_wrt_exp using solve [auto] : lngen. 
 
-(* begin hide *)
-
-Lemma open_exp_wrt_exp_rec_close_exp_wrt_exp_rec_mutual :
-(forall n1 (e1 : exp n1) x1,
-  open_exp_wrt_exp_rec (var_f x1) (close_exp_wrt_exp_rec x1 e1) = e1).
-Proof.
-intros.
-dependent induction e1; simp close_exp_wrt_exp_rec.
-+ funelim (increase_fin f); simp_stlc; default_simp.
-+ default_simp. simp_stlc. default_simp.
-+ simp_stlc. default_simp.
-+ simp_stlc. default_simp.
-Qed.
-
-(* end hide *)
-
-(* begin hide *)
-
-Lemma open_exp_wrt_exp_rec_close_exp_wrt_exp_rec :
-forall n1 (e1 : exp n1) x1,
-  open_exp_wrt_exp_rec (var_f x1) (close_exp_wrt_exp_rec x1 e1) = e1.
-Proof.
-pose proof open_exp_wrt_exp_rec_close_exp_wrt_exp_rec_mutual as H; intuition eauto.
-Qed.
-
-#[global] Hint Resolve open_exp_wrt_exp_rec_close_exp_wrt_exp_rec : lngen.
-Hint Rewrite open_exp_wrt_exp_rec_close_exp_wrt_exp_rec using solve [auto] : lngen.
-
-(* end hide *)
 
 Lemma open_exp_wrt_exp_close_exp_wrt_exp :
-forall e1 x1,
-  open_exp_wrt_exp (close_exp_wrt_exp x1 e1) (var_f x1) = e1.
+(forall n1 (e1 : exp n1) x1,
+  open_exp_wrt_exp (var_f x1) (close_exp_wrt_exp x1 e1) = e1).
 Proof.
-unfold close_exp_wrt_exp; unfold open_exp_wrt_exp; default_simp.
+  intros n1 e1. dependent induction e1; default_simp.
 Qed.
 
 #[global] Hint Resolve open_exp_wrt_exp_close_exp_wrt_exp : lngen.
 Hint Rewrite open_exp_wrt_exp_close_exp_wrt_exp using solve [auto] : lngen.
 
-(* begin hide *)
 
-Lemma open_exp_wrt_exp_rec_inj_mutual :
+Lemma open_exp_wrt_exp_inj :
 (forall n1 (e2 e1:exp (S n1)) x1,
   x1 `notin` fv_exp e2 ->
   x1 `notin` fv_exp e1 ->
-  open_exp_wrt_exp_rec (var_f x1) e2 = open_exp_wrt_exp_rec (var_f x1) e1 ->
+  open_exp_wrt_exp (var_f x1) e2 = open_exp_wrt_exp (var_f x1) e1 ->
   e2 = e1).
 Proof.
- intros k e1 e2 x1 FV1 FV2. 
+ intros k e2 e1 x1 FV1 FV2. 
  remember (var_f x1) as u.
- funelim (open_exp_wrt_exp_rec u e1). 
- all: simp open_exp_wrt_exp_rec.
+ funelim (open_exp_wrt_exp u e2). 
+ all: simp open_exp_wrt_exp.
  all: intros h.
  all: match goal with [ |- _ = ?e ] => dependent elimination e end.
- all: simp open_exp_wrt_exp_rec in h.
+ all: simp open_exp_wrt_exp in h.
  all: noconf h.
- all: try destruct (decrease_fin k f) eqn:E1.
- all: try destruct (decrease_fin k f0) eqn:E2.
+ all: try destruct_option. 
+ all: try destruct_option. 
  all: try noconf h.
  all: simpl in FV1; simpl in FV2.
- all: try solve [f_equal; eauto].
- all: try (rewrite <- E2 in E1; apply decrease_fin_inj in E1; f_equal; auto).
- all: fsetdec.
-Qed.
-
-(* end hide *)
-
-(* begin hide *)
-
-Lemma open_exp_wrt_exp_rec_inj :
-forall n1 (e2 e1 : exp (S n1)) x1,
-  x1 `notin` fv_exp e2 ->
-  x1 `notin` fv_exp e1 ->
-  open_exp_wrt_exp_rec (var_f x1) e2 = open_exp_wrt_exp_rec (var_f x1) e1 ->
-  e2 = e1.
-Proof.
-pose proof open_exp_wrt_exp_rec_inj_mutual as H; intuition eauto.
-Qed.
-
-Hint Immediate open_exp_wrt_exp_rec_inj : lngen.
-
-(* end hide *)
-
-Lemma open_exp_wrt_exp_inj :
-forall e2 e1 x1,
-  x1 `notin` fv_exp e2 ->
-  x1 `notin` fv_exp e1 ->
-  open_exp_wrt_exp e2 (var_f x1) = open_exp_wrt_exp e1 (var_f x1) ->
-  e2 = e1.
-Proof.
-unfold open_exp_wrt_exp; eauto with lngen.
+ all: default_simp. 
+ all: try (rewrite <- EQ0 in EQ; apply decrease_fin_inj in EQ).
+ all: eauto.
 Qed.
 
 Hint Immediate open_exp_wrt_exp_inj : lngen.
-
-
-(* *********************************************************************** *)
-(** * Theorems about [lc] *)
-
-(*
-Ltac default_auto ::= auto with lngen brute_force; tauto.
-Ltac default_autorewrite ::= autorewrite with lngen.
-
-(* begin hide *)
-
-Lemma degree_exp_wrt_exp_of_lc_exp_mutual :
-(forall e1,
-  lc_exp e1 ->
-  degree_exp_wrt_exp 0 e1).
-Proof.
-apply_mutual_ind lc_exp_mutind;
-intros;
-let x1 := fresh "x1" in pick_fresh x1;
-repeat (match goal with
-          | H1 : _, H2 : _ |- _ => specialize H1 with H2
-        end);
-default_simp; eauto with lngen.
-Qed.
-
-(* end hide *)
-
-Lemma degree_exp_wrt_exp_of_lc_exp :
-forall e1,
-  lc_exp e1 ->
-  degree_exp_wrt_exp 0 e1.
-Proof.
-pose proof degree_exp_wrt_exp_of_lc_exp_mutual as H; intuition eauto.
-Qed.
-
-#[global] Hint Resolve degree_exp_wrt_exp_of_lc_exp : lngen.
-
-(* begin hide *)
-
-Lemma lc_exp_of_degree_size_mutual :
-forall i1,
-(forall e1,
-  size_exp e1 = i1 ->
-  degree_exp_wrt_exp 0 e1 ->
-  lc_exp e1).
-Proof.
-intros i1; pattern i1; apply lt_wf_rec;
-clear i1; intros i1 H1;
-apply_mutual_ind exp_mutind;
-default_simp;
-(* non-trivial cases *)
-constructor; default_simp; eapply_first_lt_hyp;
-(* instantiate the size *)
-match goal with
-  | |- _ = _ => reflexivity
-  | _ => idtac
-end;
-instantiate;
-(* everything should be easy now *)
-default_simp.
-Qed.
-
-(* end hide *)
-
-Lemma lc_exp_of_degree :
-forall e1,
-  degree_exp_wrt_exp 0 e1 ->
-  lc_exp e1.
-Proof.
-intros e1; intros;
-pose proof (lc_exp_of_degree_size_mutual (size_exp e1));
-intuition eauto.
-Qed.
-
-#[global] Hint Resolve lc_exp_of_degree : lngen.
-
-Ltac typ_lc_exists_tac :=
-  repeat (match goal with
-            | H : _ |- _ =>
-              fail 1
-          end).
-
-Ltac exp_lc_exists_tac :=
-  repeat (match goal with
-            | H : _ |- _ =>
-              let J1 := fresh in pose proof H as J1; apply degree_exp_wrt_exp_of_lc_exp in J1; clear H
-          end).
-
-Lemma lc_abs_exists :
-forall x1 e1,
-  lc_exp (open_exp_wrt_exp e1 (var_f x1)) ->
-  lc_exp (abs e1).
-Proof.
-intros; exp_lc_exists_tac; eauto with lngen.
-Qed.
-
-Hint Extern 1 (lc_exp (abs _)) =>
-  let x1 := fresh in
-  pick_fresh x1;
-  apply (lc_abs_exists x1).
-
-Lemma lc_body_exp_wrt_exp :
-forall e1 e2,
-  body_exp_wrt_exp e1 ->
-  lc_exp e2 ->
-  lc_exp (open_exp_wrt_exp e1 e2).
-Proof.
-unfold body_exp_wrt_exp;
-default_simp;
-let x1 := fresh "x" in
-pick_fresh x1;
-specialize_all x1;
-exp_lc_exists_tac;
-eauto with lngen.
-Qed.
-
-#[global] Hint Resolve lc_body_exp_wrt_exp : lngen.
-
-Lemma lc_body_abs_1 :
-forall e1,
-  lc_exp (abs e1) ->
-  body_exp_wrt_exp e1.
-Proof.
-default_simp.
-Qed.
-
-#[global] Hint Resolve lc_body_abs_1 : lngen.
-*)
 
 (* *********************************************************************** *)
 (** * More theorems about [open] and [close] *)
 
 Ltac default_auto ::= auto with lngen; tauto.
-Ltac default_autorewrite ::= fail.
+Ltac default_autorewrite ::= simp_stlc.
 
-(* begin hide *)
-
-Lemma close_exp_wrt_exp_rec_degree_exp_wrt_exp_mutual :
+Lemma close_exp_wrt_exp_weaken_exp :
 (forall n1 (e1 : exp n1) x1,
   x1 `notin` fv_exp e1 ->
-  close_exp_wrt_exp_rec x1 e1 = weaken_exp e1).
+  close_exp_wrt_exp x1 e1 = weaken_exp e1).
 Proof.
 intros.
-dependent induction e1; simp_stlc; default_simp.
+dependent induction e1; default_simp.
 Qed.
 
-(* end hide *)
+#[global] Hint Resolve close_exp_wrt_exp_weaken_exp : lngen.
+Hint Rewrite close_exp_wrt_exp_weaken_exp using solve [auto] : lngen.
 
-(* begin hide *)
-
-Lemma close_exp_wrt_exp_rec_degree_exp_wrt_exp :
-forall n1 (e1 : exp n1) x1,
-  x1 `notin` fv_exp e1 ->
-  close_exp_wrt_exp_rec x1 e1 = weaken_exp e1.
-Proof.
-pose proof close_exp_wrt_exp_rec_degree_exp_wrt_exp_mutual as H; intuition eauto.
-Qed.
-
-#[global] Hint Resolve close_exp_wrt_exp_rec_degree_exp_wrt_exp : lngen.
-Hint Rewrite close_exp_wrt_exp_rec_degree_exp_wrt_exp using solve [auto] : lngen.
-
-(* end hide *)
-
-Lemma close_exp_wrt_exp_lc_exp :
-forall (e1 : exp 0) x1,
-  x1 `notin` fv_exp e1 ->
-  close_exp_wrt_exp x1 e1 = weaken_exp e1.
-Proof.
-unfold close_exp_wrt_exp; default_simp.
-Qed.
-
-#[global] Hint Resolve close_exp_wrt_exp_lc_exp : lngen.
-Hint Rewrite close_exp_wrt_exp_lc_exp using solve [auto] : lngen.
-
-(* begin hide *)
-
-Lemma open_exp_wrt_exp_rec_weaken_exp_mutual :
+Lemma open_exp_wrt_exp_weaken_exp :
 forall n1 (e2 : exp n1) e1,
-  open_exp_wrt_exp_rec e1 (weaken_exp e2) = e2.
+  open_exp_wrt_exp e1 (weaken_exp e2) = e2.
 Proof.
-intros n1 e2 e1.
-funelim (weaken_exp e2).
-all: simp_stlc; default_simp.
+intros n1 e2.
+funelim (weaken_exp e2); default_simp.
 Qed.
-
-(* end hide *)
-
-(* begin hide *)
-
-Lemma open_exp_wrt_exp_rec_degree_exp_wrt_exp :
-forall n1 (e2 : exp n1) e1,
-  open_exp_wrt_exp_rec e1 (weaken_exp e2) = e2.
-Proof.
-pose proof open_exp_wrt_exp_rec_weaken_exp_mutual as H; intuition eauto.
-Qed.
-
-#[global] Hint Resolve open_exp_wrt_exp_rec_degree_exp_wrt_exp : lngen.
-Hint Rewrite open_exp_wrt_exp_rec_degree_exp_wrt_exp using solve [auto] : lngen.
-
-(* end hide *)
-
-Lemma open_exp_wrt_exp_lc_exp :
-forall e2 e1,
-  open_exp_wrt_exp (weaken_exp e2) e1 = e2.
-Proof.
-unfold open_exp_wrt_exp; default_simp.
-Qed.
-
-#[global] Hint Resolve open_exp_wrt_exp_lc_exp : lngen.
-Hint Rewrite open_exp_wrt_exp_lc_exp using solve [auto] : lngen.
+#[global] Hint Resolve open_exp_wrt_exp_weaken_exp : lngen.
+Hint Rewrite open_exp_wrt_exp_weaken_exp using solve [auto] : lngen.
 
 
 (* *********************************************************************** *)
 (** * Theorems about [fv] *)
 
 Ltac default_auto ::= auto with set lngen; tauto.
-Ltac default_autorewrite ::= autorewrite with lngen.
-
-(* begin hide *)
-
-Lemma fv_exp_close_exp_wrt_exp_rec_mutual :
-(forall n1 (e1 : exp n1) x1,
-  fv_exp (close_exp_wrt_exp_rec x1 e1) [=] remove x1 (fv_exp e1)).
-Proof.
-dependent induction e1; intros;
-simp_stlc;
-default_simp; fsetdec. 
-Qed.
-
-(* end hide *)
-
-(* begin hide *)
-
-Lemma fv_exp_close_exp_wrt_exp_rec :
-forall n1 (e1 : exp n1) x1,
-  fv_exp (close_exp_wrt_exp_rec x1 e1) [=] remove x1 (fv_exp e1).
-Proof.
-pose proof fv_exp_close_exp_wrt_exp_rec_mutual as H; intuition eauto.
-Qed.
-
-#[global] Hint Resolve fv_exp_close_exp_wrt_exp_rec : lngen.
-Hint Rewrite fv_exp_close_exp_wrt_exp_rec using solve [auto] : lngen.
-
-(* end hide *)
+Ltac default_autorewrite ::= autorewrite with lngen; simp_stlc.
 
 Lemma fv_exp_close_exp_wrt_exp :
-forall e1 x1,
-  fv_exp (close_exp_wrt_exp x1 e1) [=] remove x1 (fv_exp e1).
+(forall n1 (e1 : exp n1) x1,
+  fv_exp (close_exp_wrt_exp x1 e1) [=] remove x1 (fv_exp e1)).
 Proof.
-  simp_stlc; default_simp.
+dependent induction e1; default_simp; fsetdec. 
 Qed.
 
 #[global] Hint Resolve fv_exp_close_exp_wrt_exp : lngen.
 Hint Rewrite fv_exp_close_exp_wrt_exp using solve [auto] : lngen.
 
-(* begin hide *)
-
-Lemma fv_exp_open_exp_wrt_exp_rec_lower_mutual :
+Lemma fv_exp_open_exp_wrt_exp_lower :
 (forall n1 (e1 : exp (S n1)) (e2 : exp n1),
-  fv_exp e1 [<=] fv_exp (open_exp_wrt_exp_rec e2 e1)).
+  fv_exp e1 [<=] fv_exp (open_exp_wrt_exp e2 e1)).
 Proof.
   intros n1 e1 e2.
-  funelim  (open_exp_wrt_exp_rec e2 e1); 
+  funelim  (open_exp_wrt_exp e2 e1); 
     simp_stlc;
     try destruct (decrease_fin k f); 
     default_simp; fsetdec.
-Qed.
-
-(* end hide *)
-
-(* begin hide *)
-
-Lemma fv_exp_open_exp_wrt_exp_rec_lower :
-forall n1 (e1 : exp (S n1)) (e2 : exp n1),
-  fv_exp e1 [<=] fv_exp (open_exp_wrt_exp_rec e2 e1).
-Proof.
-pose proof fv_exp_open_exp_wrt_exp_rec_lower_mutual as H; intuition eauto.
-Qed.
-
-#[global] Hint Resolve fv_exp_open_exp_wrt_exp_rec_lower : lngen.
-
-(* end hide *)
-
-Lemma fv_exp_open_exp_wrt_exp_lower :
-forall e1 e2,
-  fv_exp e1 [<=] fv_exp (open_exp_wrt_exp e1 e2).
-Proof.
-unfold open_exp_wrt_exp; default_simp.
 Qed.
 
 #[global] Hint Resolve fv_exp_open_exp_wrt_exp_lower : lngen.
 
 (* begin hide *)
 
-Lemma fv_exp_open_exp_wrt_exp_rec_upper_mutual :
+Lemma fv_exp_open_exp_wrt_exp_upper :
 (forall n1 (e1 : exp (S n1)) (e2 : exp n1),
-  fv_exp (open_exp_wrt_exp_rec e2 e1) [<=] fv_exp e2 `union` fv_exp e1).
+  fv_exp (open_exp_wrt_exp e2 e1) [<=] fv_exp e2 `union` fv_exp e1).
 Proof.
   intros n1 e1 e2.
-  funelim (open_exp_wrt_exp_rec e2 e1); simp_stlc. 
+  funelim (open_exp_wrt_exp e2 e1); simp_stlc. 
   all: try destruct decrease_fin; default_simp. 
-  move:H. simp_stlc. 
-Qed.
-(* end hide *)
-
-(* begin hide *)
-
-Lemma fv_exp_open_exp_wrt_exp_rec_upper :
-forall n (e1 : exp (S n)) (e2 : exp n),
-  fv_exp (open_exp_wrt_exp_rec e2 e1) [<=] fv_exp e2 `union` fv_exp e1.
-Proof.
-pose proof fv_exp_open_exp_wrt_exp_rec_upper_mutual as H; intuition eauto.
-Qed.
-
-#[global] Hint Resolve fv_exp_open_exp_wrt_exp_rec_upper : lngen.
-
-(* end hide *)
-
-Lemma fv_exp_open_exp_wrt_exp_upper :
-forall e1 e2,
-  fv_exp (open_exp_wrt_exp e1 e2) [<=] fv_exp e2 `union` fv_exp e1.
-Proof.
-unfold open_exp_wrt_exp; default_simp.
+  simp lngen in H.
 Qed.
 
 #[global] Hint Resolve fv_exp_open_exp_wrt_exp_upper : lngen.
 
-(* begin hide *)
-
-Lemma fv_exp_subst_exp_fresh_mutual :
-(forall e1 e2 x1,
+Lemma fv_exp_subst_exp_wrt_exp_fresh :
+(forall n1 (e1 : exp n1) e2 x1,
   x1 `notin` fv_exp e1 ->
-  fv_exp (subst_exp e2 x1 e1) [=] fv_exp e1).
+  fv_exp (subst_exp_wrt_exp e2 x1 e1) [=] fv_exp e1).
 Proof.
-intros e1 e2 x1.
-simp_stlc. generalize dependent 0.
-dependent induction e1.
-all: intros e2.
-all: simp_stlc. 
-all: default_simp.
+intros n1 e1.
+dependent induction e1; default_simp.
 Qed.
 
-(* end hide *)
+#[global] Hint Resolve fv_exp_subst_exp_wrt_exp_fresh : lngen.
+Hint Rewrite fv_exp_subst_exp_wrt_exp_fresh using solve [auto] : lngen.
 
-Lemma fv_exp_subst_exp_fresh :
-forall e1 e2 x1,
-  x1 `notin` fv_exp e1 ->
-  fv_exp (subst_exp e2 x1 e1) [=] fv_exp e1.
+Lemma fv_exp_subst_exp_wrt_exp_lower :
+(forall n1 (e1 : exp n1) e2 x1,
+  remove x1 (fv_exp e1) [<=] fv_exp (subst_exp_wrt_exp e2 x1 e1)).
 Proof.
-pose proof fv_exp_subst_exp_fresh_mutual as H; intuition eauto.
-Qed.
-
-#[global] Hint Resolve fv_exp_subst_exp_fresh : lngen.
-Hint Rewrite fv_exp_subst_exp_fresh using solve [auto] : lngen.
-
-(* begin hide *)
-
-Lemma fv_exp_subst_exp_lower_mutual :
-(forall e1 e2 x1,
-  remove x1 (fv_exp e1) [<=] fv_exp (subst_exp e2 x1 e1)).
-Proof.
-intros e1 e2 x1.
-simp subst_exp. generalize dependent 0.
-dependent induction e1.
-all: intros e2.
-all: simp_stlc. 
-all: default_simp.
+intros n1 e1.
+dependent induction e1; default_simp.
 fsetdec.
 Qed.
 
-(* end hide *)
-
-Lemma fv_exp_subst_exp_lower :
-forall e1 e2 x1,
-  remove x1 (fv_exp e1) [<=] fv_exp (subst_exp e2 x1 e1).
-Proof.
-pose proof fv_exp_subst_exp_lower_mutual as H; intuition eauto.
-Qed.
-
-#[global] Hint Resolve fv_exp_subst_exp_lower : lngen.
+#[global] Hint Resolve fv_exp_subst_exp_wrt_exp_lower : lngen.
 
 (* begin hide *)
 
-Lemma fv_exp_subst_exp_notin_mutual :
-(forall e1 e2 x1 x2,
+Lemma fv_exp_subst_exp_wrt_exp_notin :
+(forall n1 (e1 : exp n1) e2 x1 x2,
   x2 `notin` fv_exp e1 ->
   x2 `notin` fv_exp e2 ->
-  x2 `notin` fv_exp (subst_exp e2 x1 e1)).
+  x2 `notin` fv_exp (subst_exp_wrt_exp e2 x1 e1)).
 Proof.
-intros e1 e2 x1.
-simp subst_exp. generalize dependent 0.
-dependent induction e1.
-all: intros e2.
-all: simp_stlc. 
-all: default_simp.
+intros n1 e1.
+dependent induction e1; default_simp.
 eapply IHe1. auto. simp_stlc.
 Qed.
 
-(* end hide *)
+#[global] Hint Resolve fv_exp_subst_exp_wrt_exp_notin : lngen.
 
-Lemma fv_exp_subst_exp_notin :
-forall e1 e2 x1 x2,
-  x2 `notin` fv_exp e1 ->
-  x2 `notin` fv_exp e2 ->
-  x2 `notin` fv_exp (subst_exp e2 x1 e1).
+Lemma fv_exp_subst_exp_wrt_exp_upper :
+(forall n1 (e1 : exp n1) e2 x1,
+  fv_exp (subst_exp_wrt_exp e2 x1 e1) [<=] fv_exp e2 `union` remove x1 (fv_exp e1)).
 Proof.
-pose proof fv_exp_subst_exp_notin_mutual as H; intuition eauto.
-Qed.
-
-#[global] Hint Resolve fv_exp_subst_exp_notin : lngen.
-
-(* begin hide *)
-
-Lemma fv_exp_subst_exp_upper_mutual :
-(forall e1 e2 x1,
-  fv_exp (subst_exp e2 x1 e1) [<=] fv_exp e2 `union` remove x1 (fv_exp e1)).
-Proof.
-intros e1 e2 x1.
-simp subst_exp. generalize dependent 0.
-dependent induction e1.
-all: intros e2.
-all: simp_stlc. 
-all: default_simp.
+intros n1 e1.
+dependent induction e1; default_simp.
 fsetdec.
 specialize (IHe1 (weaken_exp e2)).
-move:IHe1. simp weaken_exp.
+simp weaken_exp in IHe1.
 Qed.
 
-(* end hide *)
-
-Lemma fv_exp_subst_exp_upper :
-forall e1 e2 x1,
-  fv_exp (subst_exp e2 x1 e1) [<=] fv_exp e2 `union` remove x1 (fv_exp e1).
-Proof.
-pose proof fv_exp_subst_exp_upper_mutual as H; intuition eauto.
-Qed.
-
-#[global] Hint Resolve fv_exp_subst_exp_upper : lngen.
+#[global] Hint Resolve fv_exp_subst_exp_wrt_exp_upper : lngen.
 
 
 (* *********************************************************************** *)
 (** * Theorems about [subst] *)
 
 Ltac default_auto ::= auto with lngen brute_force; tauto.
-Ltac default_autorewrite ::= autorewrite with lngen.
-
-(* begin hide *)
-
-(* We need to make subst take an exp 0 always (and then weaken at the bottom) in order to state this lemma *)
-
-(*
-Lemma subst_exp_close_exp_wrt_exp_rec_mutual :
-forall {n1} (e2 : exp n1) (e1 : exp n1) x1 x2,
-  x1 <> x2 ->
-  x2 `notin` fv_exp e1 ->
-  subst_exp_rec e1 x1 (close_exp_wrt_exp_rec x2 e2) = close_exp_wrt_exp_rec x2 (subst_exp_rec e1 x1 e2).
-Proof.
-intros. 
-funelim (subst_exp_rec e1 x1 e2).
-all: simp_stlc.
-all: default_simp.
-Qed.
-
-(* end hide *)
-
-Lemma subst_exp_close_exp_wrt_exp_rec :
-forall e2 e1 x1 x2 n1,
-  degree_exp_wrt_exp n1 e1 ->
-  x1 <> x2 ->
-  x2 `notin` fv_exp e1 ->
-  subst_exp e1 x1 (close_exp_wrt_exp_rec n1 x2 e2) = close_exp_wrt_exp_rec n1 x2 (subst_exp e1 x1 e2).
-Proof.
-pose proof subst_exp_close_exp_wrt_exp_rec_mutual as H; intuition eauto.
-Qed.
-
-#[global] Hint Resolve subst_exp_close_exp_wrt_exp_rec : lngen.
+Ltac default_autorewrite ::= simp_stlc; autorewrite with lngen.
 
 Lemma subst_exp_close_exp_wrt_exp :
-forall e2 e1 x1 x2,
-  lc_exp e1 ->  x1 <> x2 ->
+forall n1 (e2 : exp n1) (e1 : exp n1) x1 x2,
+  x1 <> x2 ->
   x2 `notin` fv_exp e1 ->
-  subst_exp e1 x1 (close_exp_wrt_exp x2 e2) = close_exp_wrt_exp x2 (subst_exp e1 x1 e2).
+  subst_exp_wrt_exp (weaken_exp e1) x1 (close_exp_wrt_exp x2 e2) =
+        close_exp_wrt_exp x2 (subst_exp_wrt_exp e1 x1 e2).
 Proof.
-unfold close_exp_wrt_exp; default_simp.
+intros n1 e2.
+dependent induction e2. 
+all: default_simp.
+specialize (IHe2 (weaken_exp e1)).
+eapply IHe2; simp_stlc; auto.
 Qed.
+
 
 #[global] Hint Resolve subst_exp_close_exp_wrt_exp : lngen.
 
-(* begin hide *)
 
-Lemma subst_exp_degree_exp_wrt_exp_mutual :
-(forall e1 e2 x1 n1,
-  degree_exp_wrt_exp n1 e1 ->
-  degree_exp_wrt_exp n1 e2 ->
-  degree_exp_wrt_exp n1 (subst_exp e2 x1 e1)).
-Proof.
-apply_mutual_ind exp_mutind;
-default_simp.
-Qed.
-
-(* end hide *)
-
-Lemma subst_exp_degree_exp_wrt_exp :
-forall e1 e2 x1 n1,
-  degree_exp_wrt_exp n1 e1 ->
-  degree_exp_wrt_exp n1 e2 ->
-  degree_exp_wrt_exp n1 (subst_exp e2 x1 e1).
-Proof.
-pose proof subst_exp_degree_exp_wrt_exp_mutual as H; intuition eauto.
-Qed.
-
-#[global] Hint Resolve subst_exp_degree_exp_wrt_exp : lngen.
-*)
-
-(* begin hide *)
-
-Lemma subst_exp_fresh_eq_mutual :
-(forall n (e2 e1 : exp n) x1,
+Lemma subst_exp_wrt_exp_fresh_eq :
+forall n1 (e2 : exp n1) e1 x1,
   x1 `notin` fv_exp e2 ->
-  subst_exp_rec e1 x1 e2 = e2).
+  subst_exp_wrt_exp e1 x1 e2 = e2.
 Proof.
-intros n e2 e1 x1.
-dependent induction e2.
-all: simp_stlc. 
-all: default_simp.
+  intros. 
+  dependent induction e2; default_simp.
 Qed.
 
-#[global] Hint Resolve subst_exp_fresh_eq_mutual : lngen.
-Hint Rewrite subst_exp_fresh_eq_mutual using solve [auto] : lngen.
+#[global] Hint Resolve subst_exp_wrt_exp_fresh_eq : lngen.
+Hint Rewrite subst_exp_wrt_exp_fresh_eq using solve [auto] : lngen.
 
-
-(* end hide *)
-
-Lemma subst_exp_fresh_eq :
-forall e2 e1 x1,
-  x1 `notin` fv_exp e2 ->
-  subst_exp e1 x1 e2 = e2.
-Proof.
-  intros. simp_stlc.
-pose proof subst_exp_fresh_eq_mutual as h; intuition eauto.
-Qed.
-
-#[global] Hint Resolve subst_exp_fresh_eq : lngen.
-Hint Rewrite subst_exp_fresh_eq using solve [auto] : lngen.
-
-(* begin hide *)
-
-Lemma subst_exp_fresh_same_mutual :
-(forall e2 e1 x1,
+Lemma subst_exp_wrt_exp_fresh_same :
+(forall n1 (e2 : exp n1) e1 x1,
   x1 `notin` fv_exp e1 ->
-  x1 `notin` fv_exp (subst_exp e1 x1 e2)).
+  x1 `notin` fv_exp (subst_exp_wrt_exp e1 x1 e2)).
 Proof.
-intros e2 e1 x1.
-simp subst_exp. generalize dependent 0.
-dependent induction e2.
-all: intros e1.
-all: simp_stlc. 
-all: default_simp.
-specialize (IHe2 (weaken_exp e1)). 
+intros n1 e2.
+dependent induction e2; default_simp.
+specialize (IHe2 (weaken_exp e1)).
 eapply IHe2. simp_stlc.
 Qed.
 
+#[global] Hint Resolve subst_exp_wrt_exp_fresh_same : lngen.
 
-(* end hide *)
-
-Lemma subst_exp_fresh_same :
-forall e2 e1 x1,
-  x1 `notin` fv_exp e1 ->
-  x1 `notin` fv_exp (subst_exp e1 x1 e2).
-Proof.
-pose proof subst_exp_fresh_same_mutual as H; intuition eauto.
-Qed.
-
-#[global] Hint Resolve subst_exp_fresh_same : lngen.
-
-(* begin hide *)
-
-Lemma subst_exp_fresh_mutual :
-(forall e2 e1 x1 x2,
+Lemma subst_exp_wrt_exp_fresh :
+(forall n1 (e2:exp n1) e1 x1 x2,
   x1 `notin` fv_exp e2 ->
   x1 `notin` fv_exp e1 ->
-  x1 `notin` fv_exp (subst_exp e1 x2 e2)).
+  x1 `notin` fv_exp (subst_exp_wrt_exp e1 x2 e2)).
 Proof.
-intros e2 e1 x1 x2.
-simp subst_exp. generalize dependent 0.
-dependent induction e2.
-all: intros e1.
-all: simp_stlc. 
-all: default_simp.
-specialize (IHe2 (weaken_exp e1)); eapply IHe2; simp_stlc.
+intros n1 e2.
+dependent induction e2; default_simp.
 Qed.
 
-(* end hide *)
+#[global] Hint Resolve subst_exp_wrt_exp_fresh : lngen.
 
-Lemma subst_exp_fresh :
-forall e2 e1 x1 x2,
-  x1 `notin` fv_exp e2 ->
-  x1 `notin` fv_exp e1 ->
-  x1 `notin` fv_exp (subst_exp e1 x2 e2).
-Proof.
-pose proof subst_exp_fresh_mutual as H; intuition eauto.
-Qed.
-
-#[global] Hint Resolve subst_exp_fresh : lngen.
-
-(*
-Lemma subst_exp_lc_exp :
-forall e1 e2 x1,
-  lc_exp e1 ->
-  lc_exp e2 ->
-  lc_exp (subst_exp e2 x1 e1).
-Proof.
-default_simp.
-Qed.
-
-#[global] Hint Resolve subst_exp_lc_exp : lngen.
-*)
-
-Lemma subst_exp_rec_weaken_exp : forall n (e1 : exp n) x1 u,
- subst_exp_rec (weaken_exp e1) x1 (weaken_exp u) = weaken_exp (subst_exp_rec e1 x1 u).
+Lemma subst_exp_wrt_exp_weaken_exp : 
+  forall n (e1 : exp n) x1 u,
+    weaken_exp (subst_exp_wrt_exp e1 x1 u) = 
+    subst_exp_wrt_exp (weaken_exp e1) x1 (weaken_exp u).
 Proof.
   intros.
   funelim (weaken_exp u); simp_stlc; default_simp.
 Qed.
 
-#[global] Hint Resolve subst_exp_rec_weaken_exp : lngen.
-Hint Rewrite subst_exp_rec_weaken_exp : lngen.
+#[global] Hint Resolve subst_exp_wrt_exp_weaken_exp : lngen.
+Hint Rewrite subst_exp_wrt_exp_weaken_exp : lngen.
 
-
-(* begin hide *)
-
-Lemma subst_exp_open_exp_wrt_exp_rec_mutual :
+(* SCW: this one might be simpler if we only substitute 
+   locally closed terms *)
+Lemma subst_exp_open_exp_wrt_exp :
 (forall n1 (e1 : exp n1) e2 (e3 : exp (S n1)) x1,
-  subst_exp_rec e1 x1 (open_exp_wrt_exp_rec e2 e3) = open_exp_wrt_exp_rec (subst_exp_rec e1 x1 e2) (subst_exp_rec (weaken_exp e1) x1 e3)).
+  subst_exp_wrt_exp e1 x1 (open_exp_wrt_exp e2 e3) =
+    open_exp_wrt_exp (subst_exp_wrt_exp e1 x1 e2) 
+                         (subst_exp_wrt_exp (weaken_exp e1) x1 e3)).
 Proof.
 intros n1 e1 e2 e3 x1.
-funelim (open_exp_wrt_exp_rec e2 e3).
-all: simp_stlc. 
+funelim (open_exp_wrt_exp e2 e3).
 all: default_simp.
 destruct (decrease_fin k f) eqn:E1.
-simp_stlc. auto. auto.
-rewrite H.
+default_simp.
 default_simp.
 Qed.
-
-(* end hide *)
-
-(* begin hide *)
-
-(* SCW: this one also might be simpler if we only substitute 
-   locally closed terms *)
-Lemma subst_exp_open_exp_wrt_exp_rec :
-forall n1 (e3 : exp (S n1)) e1 e2 x1,
-  subst_exp_rec e1 x1 (open_exp_wrt_exp_rec e2 e3) = 
-    open_exp_wrt_exp_rec (subst_exp_rec e1 x1 e2) 
-                         (subst_exp_rec (weaken_exp e1) x1 e3).
-Proof.
-pose proof subst_exp_open_exp_wrt_exp_rec_mutual as H; intuition eauto.
-Qed.
-
-#[global] Hint Resolve subst_exp_open_exp_wrt_exp_rec : lngen.
-
-(* end hide *)
-
-Lemma subst_exp_open_exp_wrt_exp :
-forall e3 e1 e2 x1,
-  subst_exp e1 x1 (open_exp_wrt_exp e3 e2) = 
-    open_exp_wrt_exp (subst_exp_rec (weaken_exp e1) x1 e3) (subst_exp e1 x1 e2).
-Proof.
- intros.
- simp subst_exp.
- simp_stlc.
- default_simp.
-Admitted.
 
 #[global] Hint Resolve subst_exp_open_exp_wrt_exp : lngen.
 
 Lemma subst_exp_open_exp_wrt_exp_var :
-forall e2 e1 x1 x2,
+forall n1 (e2 : exp (S n1)) e1 x1 x2,
   x1 <> x2 ->
-  open_exp_wrt_exp (subst_exp_rec (weaken_exp e1) x1 e2) (var_f x2) = 
-    subst_exp e1 x1 (open_exp_wrt_exp e2 (var_f x2)).
+  open_exp_wrt_exp (var_f x2) (subst_exp_wrt_exp (weaken_exp e1) x1 e2) = 
+    subst_exp_wrt_exp e1 x1 (open_exp_wrt_exp (var_f x2) e2).
 Proof.
-intros; rewrite subst_exp_open_exp_wrt_exp; default_simp.
-Qed.
+intros; default_simp.
+Admitted.
 
 #[global] Hint Resolve subst_exp_open_exp_wrt_exp_var : lngen.
 
 (* begin hide *)
 
-Lemma subst_exp_spec_rec_mutual :
+Lemma subst_exp_wrt_exp_spec :
 (forall n (e1 e2 : exp n) x1,
-  subst_exp_rec e2 x1 e1 = open_exp_wrt_exp_rec e2 (close_exp_wrt_exp_rec  x1 e1)).
+  subst_exp_wrt_exp e2 x1 e1 = open_exp_wrt_exp e2 (close_exp_wrt_exp  x1 e1)).
 Proof.
 intros n e1 e2 x1.
 dependent induction e1.
-all: simp_stlc. 
 all: default_simp.
-simp_stlc. auto.
 Qed.
 
-
-(* end hide *)
+#[global] Hint Resolve subst_exp_wrt_exp_spec : lngen.
 
 (* begin hide *)
 
-Lemma subst_exp_spec_rec :
-forall n (e1 e2 : exp n) x1,
-  subst_exp_rec e2 x1 e1 = open_exp_wrt_exp_rec e2 (close_exp_wrt_exp_rec x1 e1).
-Proof.
-pose proof subst_exp_spec_rec_mutual as H; intuition eauto.
-Qed.
-
-#[global] Hint Resolve subst_exp_spec_rec : lngen.
-
-(* end hide *)
-
-Lemma subst_exp_spec :
-forall e1 e2 x1,
-  subst_exp e2 x1 e1 = open_exp_wrt_exp (close_exp_wrt_exp x1 e1) e2.
-Proof.
-intros. simp_stlc. default_simp.
-Qed.
-
-#[global] Hint Resolve subst_exp_spec : lngen.
-
-(* begin hide *)
-
-Lemma subst_exp_subst_exp_mutual :
+Lemma subst_exp_wrt_exp_subst_exp_wrt_exp :
 (forall n (e1 e2 e3 : exp n) x2 x1,
   x2 `notin` fv_exp e2 ->
   x2 <> x1 ->
-  subst_exp_rec e2 x1 (subst_exp_rec e3 x2 e1) = 
-    subst_exp_rec (subst_exp_rec e2 x1 e3) x2 (subst_exp_rec e2 x1 e1)).
+  subst_exp_wrt_exp e2 x1 (subst_exp_wrt_exp e3 x2 e1) = 
+    subst_exp_wrt_exp (subst_exp_wrt_exp e2 x1 e3) x2 (subst_exp_wrt_exp e2 x1 e1)).
 Proof.
 intros n e1.
 dependent induction e1; intros.
-all: simp_stlc. 
 all: default_simp.
-all: simp_stlc. 
-all: default_simp.
-rewrite IHe1. 
-all: simp_stlc.
+rewrite IHe1; 
 default_simp.
 Qed.
 
-(* end hide *)
+#[global] Hint Resolve subst_exp_wrt_exp_subst_exp_wrt_exp : lngen.
 
-Lemma subst_exp_subst_exp :
-forall e1 e2 e3 x2 x1,
-  x2 `notin` fv_exp e2 ->
-  x2 <> x1 ->
-  subst_exp e2 x1 (subst_exp e3 x2 e1) = subst_exp (subst_exp e2 x1 e3) x2 (subst_exp e2 x1 e1).
-Proof.
-intros.
-eapply subst_exp_subst_exp_mutual. auto. auto.
-(* pose proof subst_exp_subst_exp_mutual as H; intuition eauto. *)
-Qed.
-
-#[global] Hint Resolve subst_exp_subst_exp : lngen.
-
-(* begin hide *)
-
-Lemma subst_exp_close_exp_wrt_exp_rec_open_exp_wrt_exp_rec_mutual :
+Lemma subst_exp_wrt_exp_close_exp_wrt_exp_open_exp_wrt_exp :
 (forall n1 (e2 : exp (S n1)) e1 x1 x2,
   x2 `notin` fv_exp e2 ->
   x2 `notin` fv_exp e1 ->
   x2 <> x1 ->
-  subst_exp_rec (weaken_exp e1) x1 e2 = 
-    close_exp_wrt_exp_rec x2 
-       (subst_exp_rec e1 x1 (open_exp_wrt_exp_rec (var_f x2) e2))).
+  subst_exp_wrt_exp (weaken_exp e1) x1 e2 = 
+    close_exp_wrt_exp x2 
+       (subst_exp_wrt_exp e1 x1 (open_exp_wrt_exp (var_f x2) e2))).
 Proof.
 intros n e2.
 dependent induction e2; intros.
-all: simp_stlc. 
 all: default_simp.
 all: try destruct (decrease_fin n f) eqn:E.
-all: default_simp.
-all: simp_stlc. 
 all: default_simp.
 symmetry. eauto using decrease_increase_fin.
 symmetry. eauto using decrease_to_fin.
@@ -1468,80 +493,45 @@ eapply IHe2; eauto.
 all: simp_stlc. 
 Qed.
 
-(* end hide *)
+#[global] Hint Resolve subst_exp_wrt_exp_close_exp_wrt_exp_open_exp_wrt_exp : lngen.
 
-(* begin hide *)
-
-Lemma subst_exp_close_exp_wrt_exp_rec_open_exp_wrt_exp_rec :
-forall n1 (e2 : exp (S n1)) e1 x1 x2,
-  x2 `notin` fv_exp e2 ->
-  x2 `notin` fv_exp e1 ->
-  x2 <> x1 ->
-  subst_exp_rec (weaken_exp e1) x1 e2 = close_exp_wrt_exp_rec  x2 (subst_exp_rec e1 x1 (open_exp_wrt_exp_rec (var_f x2) e2)).
-Proof.
-pose proof subst_exp_close_exp_wrt_exp_rec_open_exp_wrt_exp_rec_mutual as H; intuition eauto.
-Qed.
-
-#[global] Hint Resolve subst_exp_close_exp_wrt_exp_rec_open_exp_wrt_exp_rec : lngen.
-
-(* end hide *)
-
-Lemma subst_exp_close_exp_wrt_exp_open_exp_wrt_exp :
-forall (e2 : exp 1) (e1 : exp 0) x1 x2,
-  x2 `notin` fv_exp e2 ->
-  x2 `notin` fv_exp e1 ->
-  x2 <> x1 ->
-  subst_exp_rec (weaken_exp e1) x1 e2 =
-    close_exp_wrt_exp x2 (subst_exp_rec e1 x1 (open_exp_wrt_exp e2 (var_f x2))).
-Proof.
-unfold close_exp_wrt_exp; unfold open_exp_wrt_exp; default_simp.
-Qed.
-
-#[global] Hint Resolve subst_exp_close_exp_wrt_exp_open_exp_wrt_exp : lngen.
-
-Lemma subst_exp_abs :
+Lemma subst_exp_wrt_exp_abs :
 forall x2 (e2 : exp 1) (e1 : exp 0) x1,
   x2 `notin` fv_exp e1 `union` fv_exp e2 `union` singleton x1 ->
-  subst_exp e1 x1 (abs e2) = abs (close_exp_wrt_exp x2 (subst_exp e1 x1 (open_exp_wrt_exp e2 (var_f x2)))).
+  subst_exp_wrt_exp e1 x1 (abs e2) = 
+    abs (close_exp_wrt_exp x2 (subst_exp_wrt_exp e1 x1 (open_exp_wrt_exp (var_f x2) e2))).
 Proof.
-default_simp. simp_stlc. default_simp.
+default_simp. 
 Qed.
 
-#[global] Hint Resolve subst_exp_abs : lngen.
+#[global] Hint Resolve subst_exp_wrt_exp_abs : lngen.
 
-(* begin hide *)
-Lemma subst_exp_intro_rec :
+Lemma subst_exp_wrt_exp_intro :
 forall n1 (e1 : exp (S n1)) x1 e2,
   x1 `notin` fv_exp e1 ->
-  open_exp_wrt_exp_rec e2 e1 = subst_exp_rec e2 x1 (open_exp_wrt_exp_rec (var_f x1) e1).
+  open_exp_wrt_exp e2 e1 = subst_exp_wrt_exp e2 x1 (open_exp_wrt_exp (var_f x1) e1).
 Proof.
 dependent induction e1; default_simp.
-all: simp_stlc.
 all: try destruct decrease_fin eqn:E.
-all: simp_stlc.
 all: default_simp.
 Qed.
 
-#[global] Hint Resolve subst_exp_intro_rec : lngen.
-Hint Rewrite subst_exp_intro_rec using solve [auto] : lngen.
-
-(* end hide *)
-
-Lemma subst_exp_intro :
-forall x1 e1 e2,
-  x1 `notin` fv_exp e1 ->
-  open_exp_wrt_exp e1 e2 = subst_exp e2 x1 (open_exp_wrt_exp e1 (var_f x1)).
-Proof.
-unfold open_exp_wrt_exp; default_simp.
-simp_stlc.
-default_simp.
-Qed.
-
-#[global] Hint Resolve subst_exp_intro : lngen.
-
+#[global] Hint Resolve subst_exp_wrt_exp_intro : lngen.
+Hint Rewrite subst_exp_wrt_exp_intro using solve [auto] : lngen.
 
 (* *********************************************************************** *)
 (** * "Restore" tactics *)
 
 Ltac default_auto ::= auto; tauto.
 Ltac default_autorewrite ::= fail.
+
+
+Instance STE :  SyntaxTheory exp := {
+  size_weaken := size_exp_weaken_exp;
+  fv_weaken := fv_exp_weaken_exp;
+  size_min  := size_exp_min;
+  subst_intro := subst_exp_wrt_exp_intro;
+  subst_open_var := subst_exp_open_exp_wrt_exp_var 
+}.
+
+Opaque Syntax_exp.
